src/Init/Data/Range/Polymorphic/Lemmas.lean
@@ -6,7 +6,7 @@ Authors: Paul Reichert
 module
 
 prelude
-public import Init.Data.Iterators
+public import Init.Data.Iterators.Lemmas.Consumers.Loop
 import Init.Data.Iterators.Lemmas.Consumers.Collect
 public import Init.Data.Range.Polymorphic.Basic
 import all Init.Data.Range.Polymorphic.Basic
@@ -25,196 +25,10 @@ public section
 This file provides lemmas about `Std.PRange`.
 -/
 
-namespace Std.PRange
-open Std.Iterators
+namespace Std
+open Std.PRange Std.Iterators
 
-variable {shape : RangeShape} {α : Type u}
-
-private theorem Internal.iter_Rox_eq_iter_Rcx_of_isSome_succ? {su} [UpwardEnumerable α]
-    [SupportsUpperBound su α] [HasFiniteRanges su α]
-    [LawfulUpwardEnumerable α]
-    {lo : Bound .open α} {hi} (h : (UpwardEnumerable.succ? lo).isSome) :
-    Internal.iter (PRange.mk (shape := ⟨.open, su⟩) lo hi) =
-      Internal.iter (PRange.mk (shape := ⟨.closed, su⟩) (UpwardEnumerable.succ? lo |>.get h) hi) := by
-  simp [Internal.iter, init?]
-
-private theorem Internal.toList_eq_toList_iter {sl su} [UpwardEnumerable α]
-    [BoundedUpwardEnumerable sl α] [SupportsUpperBound su α] [HasFiniteRanges su α]
-    [LawfulUpwardEnumerable α] {r : PRange ⟨sl, su⟩ α} :
-    r.toList = (Internal.iter r).toList := by
-  rfl
-
-public theorem RangeIterator.toList_eq_match {su} [UpwardEnumerable α]
-    [SupportsUpperBound su α] [HasFiniteRanges su α]
-    [LawfulUpwardEnumerable α]
-    {it : Iter (α := RangeIterator su α) α} :
-    it.toList =  match it.internalState.next with
-      | none => []
-      | some a => if SupportsUpperBound.IsSatisfied it.internalState.upperBound a then
-          a :: (⟨⟨UpwardEnumerable.succ? a, it.internalState.upperBound⟩⟩ : Iter (α := RangeIterator su α) α).toList
-        else
-          [] := by
-  apply Eq.symm
-  rw [Iter.toList_eq_match_step, RangeIterator.step_eq_step]
-  simp only [RangeIterator.step]
-  split <;> rename_i heq
-  · simp [*]
-  · split <;> rename_i heq' <;> simp [*]
-
-public theorem toList_eq_match {sl su} [UpwardEnumerable α] [BoundedUpwardEnumerable sl α]
-    [SupportsUpperBound su α] [HasFiniteRanges su α]
-    [LawfulUpwardEnumerable α]
-    {r : PRange ⟨sl, su⟩ α} :
-    r.toList = match init? r.lower with
-      | none => []
-      | some a => if SupportsUpperBound.IsSatisfied r.upper a then
-        a :: (PRange.mk (shape := ⟨.open, su⟩) a r.upper).toList
-      else
-        [] := by
-  rw [Internal.toList_eq_toList_iter, RangeIterator.toList_eq_match]; rfl
-
-public theorem toList_Rox_eq_toList_Rcx_of_isSome_succ? {su} [UpwardEnumerable α]
-    [SupportsUpperBound su α] [HasFiniteRanges su α]
-    [LawfulUpwardEnumerable α]
-    {lo : Bound .open α} {hi} (h : (UpwardEnumerable.succ? lo).isSome) :
-    (PRange.mk (shape := ⟨.open, su⟩) lo hi).toList =
-      (PRange.mk (shape := ⟨.closed, su⟩) (UpwardEnumerable.succ? lo |>.get h) hi).toList := by
-  simp [Internal.toList_eq_toList_iter, Internal.iter_Rox_eq_iter_Rcx_of_isSome_succ?, h]
-
-@[deprecated toList_Rox_eq_toList_Rcx_of_isSome_succ? (since := "2025-08-22")]
-public theorem toList_open_eq_toList_closed_of_isSome_succ? {su} [UpwardEnumerable α]
-    [SupportsUpperBound su α] [HasFiniteRanges su α]
-    [LawfulUpwardEnumerable α]
-    {lo : Bound .open α} {hi} (h : (UpwardEnumerable.succ? lo).isSome) :
-    (PRange.mk (shape := ⟨.open, su⟩) lo hi).toList =
-      (PRange.mk (shape := ⟨.closed, su⟩) (UpwardEnumerable.succ? lo |>.get h) hi).toList :=
-  toList_Rox_eq_toList_Rcx_of_isSome_succ? h
-
-public theorem toList_eq_nil_iff {sl su} [UpwardEnumerable α]
-    [SupportsUpperBound su α] [HasFiniteRanges su α] [BoundedUpwardEnumerable sl α]
-    [LawfulUpwardEnumerable α]
-    {r : PRange ⟨sl, su⟩ α} :
-    r.toList = [] ↔
-      ¬ (∃ a, init? r.lower = some a ∧ SupportsUpperBound.IsSatisfied r.upper a) := by
-  rw [Internal.toList_eq_toList_iter]
-  rw [RangeIterator.toList_eq_match, Internal.iter]
-  simp only
-  split <;> rename_i heq <;> simp [heq]
-
-public theorem mem_toList_iff_mem {sl su} [UpwardEnumerable α]
-    [SupportsUpperBound su α] [SupportsLowerBound sl α] [HasFiniteRanges su α]
-    [BoundedUpwardEnumerable sl α] [LawfulUpwardEnumerable α]
-    [LawfulUpwardEnumerableLowerBound sl α] [LawfulUpwardEnumerableUpperBound su α]
-    {r : PRange ⟨sl, su⟩ α}
-    {a : α} : a ∈ r.toList ↔ a ∈ r := by
-  rw [Internal.toList_eq_toList_iter, Iter.mem_toList_iff_isPlausibleIndirectOutput,
-    Internal.isPlausibleIndirectOutput_iter_iff]
-
-public theorem BoundedUpwardEnumerable.init?_succ?_closed [UpwardEnumerable α]
-    [LawfulUpwardEnumerable α] {lower lower' : Bound .closed α}
-    (h : UpwardEnumerable.succ? lower = some lower') :
-    init? lower' = (init? lower).bind UpwardEnumerable.succ? := by
-  cases h : init? lower <;> rename_i ilower <;> cases h' : init? lower' <;> rename_i ilower'
-  · simp
-  · simp [init?] at h
-  · simp [init?] at h'
-  · simp_all [init?]
-
-@[deprecated BoundedUpwardEnumerable.init?_succ?_closed (since := "2025-08-22")]
-public theorem BoundedUpwardEnumerable.Closed.init?_succ [UpwardEnumerable α]
-    [LawfulUpwardEnumerable α] {lower lower' : Bound .closed α}
-    (h : UpwardEnumerable.succ? lower = some lower') :
-    init? lower' = (init? lower).bind UpwardEnumerable.succ? :=
-  init?_succ?_closed h
-
-public theorem pairwise_toList_upwardEnumerableLt {sl su} [UpwardEnumerable α]
-    [SupportsUpperBound su α] [SupportsLowerBound sl α] [HasFiniteRanges su α]
-    [BoundedUpwardEnumerable sl α] [LawfulUpwardEnumerable α]
-    [LawfulUpwardEnumerableLowerBound sl α] [LawfulUpwardEnumerableUpperBound su α]
-    {r : PRange ⟨sl, su⟩ α} :
-    r.toList.Pairwise (fun a b => UpwardEnumerable.LT a b) := by
-  rw [Internal.toList_eq_toList_iter]
-  generalize Internal.iter r = it
-  induction it using Iter.inductSteps with | step it ihy ihs
-  rw [RangeIterator.toList_eq_match]
-  repeat' split <;> (try exact .nil; done)
-  rename_i a _ _
-  apply List.Pairwise.cons
-  · intro a' ha
-    rw [Iter.mem_toList_iff_isPlausibleIndirectOutput] at ha
-    replace ha := RangeIterator.upwardEnumerableLe_of_isPlausibleIndirectOutput ha
-    simp only at ha
-    have : UpwardEnumerable.LT a ha.choose := by
-      refine ⟨0, ?_⟩
-      simp only [succMany?_succ?, succMany?_zero,
-        Option.bind_some]
-      exact ha.choose_spec.1
-    exact UpwardEnumerable.lt_of_lt_of_le this ha.choose_spec.2
-  · apply ihy (out := a)
-    simp_all [RangeIterator.isPlausibleStep_iff, RangeIterator.step]
-
-public theorem pairwise_toList_ne {sl su} [UpwardEnumerable α]
-    [SupportsUpperBound su α] [SupportsLowerBound sl α] [HasFiniteRanges su α]
-    [BoundedUpwardEnumerable sl α] [LawfulUpwardEnumerable α]
-    [LawfulUpwardEnumerableLowerBound sl α] [LawfulUpwardEnumerableUpperBound su α]
-    {r : PRange ⟨sl, su⟩ α} :
-    r.toList.Pairwise (fun a b => a ≠ b) :=
-  List.Pairwise.imp (fun hlt => UpwardEnumerable.ne_of_lt hlt) pairwise_toList_upwardEnumerableLt
-
-public theorem pairwise_toList_lt {sl su} [LT α] [UpwardEnumerable α]
-    [SupportsUpperBound su α] [SupportsLowerBound sl α] [HasFiniteRanges su α]
-    [BoundedUpwardEnumerable sl α] [LawfulUpwardEnumerable α] [LawfulUpwardEnumerableLT α]
-    [LawfulUpwardEnumerableLowerBound sl α] [LawfulUpwardEnumerableUpperBound su α]
-    {r : PRange ⟨sl, su⟩ α} :
-    r.toList.Pairwise (fun a b => a < b) :=
-  List.Pairwise.imp
-    (fun hlt => (LawfulUpwardEnumerableLT.lt_iff ..).mpr hlt) pairwise_toList_upwardEnumerableLt
-
-public theorem pairwise_toList_le {sl su} [LE α] [UpwardEnumerable α]
-    [SupportsUpperBound su α] [SupportsLowerBound sl α] [HasFiniteRanges su α]
-    [BoundedUpwardEnumerable sl α] [LawfulUpwardEnumerable α] [LawfulUpwardEnumerableLE α]
-    [LawfulUpwardEnumerableLowerBound sl α] [LawfulUpwardEnumerableUpperBound su α]
-    {r : PRange ⟨sl, su⟩ α} :
-    r.toList.Pairwise (fun a b => a ≤ b) :=
-  pairwise_toList_upwardEnumerableLt
-    |> List.Pairwise.imp UpwardEnumerable.le_of_lt
-    |> List.Pairwise.imp (fun hle => (UpwardEnumerable.le_iff ..).mpr hle)
-
-public theorem mem_Rco_succ_succ_iff [UpwardEnumerable α]
-    [LinearlyUpwardEnumerable α] [InfinitelyUpwardEnumerable α] [SupportsUpperBound .open α]
-    [SupportsLowerBound .closed α] [LawfulUpwardEnumerableLowerBound .closed α]
-    [HasFiniteRanges .open α] [LawfulUpwardEnumerable α] [LawfulOpenUpperBound α]
-    {lower : Bound .closed α} {upper : Bound .open α} {a : α} :
-    (a ∈ (succ lower)...(succ upper)) ↔ ∃ a', a = succ a' ∧ a' ∈ lower...upper := by
-  simp [Membership.mem, LawfulUpwardEnumerableLowerBound.isSatisfied_iff,
-    init?, LawfulOpenUpperBound.isSatisfied_iff_le]
-  rw [← Option.some_get (InfinitelyUpwardEnumerable.isSome_succ? _)]
-  simp only [Option.some.injEq, ← UpwardEnumerable.succ.eq_def]
-  simp
-  constructor
-  · rintro ⟨⟨n, hn⟩, h⟩
-    rw [succMany?_eq_some_iff_succMany, ← succMany_one, ← succMany_add, Nat.add_comm, succMany_add,
-      succMany_one] at hn
-    rw [← hn]
-    refine ⟨succMany n lower, rfl, ?_, ?_⟩
-    · exact ⟨n, by simp [succMany_eq_get]⟩
-    · obtain ⟨m, hm⟩ := h
-      refine ⟨m, ?_⟩
-      rw [succMany?_eq_some_iff_succMany] at hm ⊢
-      rwa [← hn, ← succMany_one, ← succMany_add, Nat.add_comm, succMany_add, succMany_one,
-        succ_eq_succ_iff] at hm
-  · rintro ⟨a', rfl, hl, hu⟩
-    simp [UpwardEnumerable.succ_le_succ_iff, UpwardEnumerable.succ_lt_succ_iff]
-    exact ⟨hl, hu⟩
-
-@[deprecated mem_Rco_succ_succ_iff (since := "2025-08-22")]
-public theorem ClosedOpen.mem_succ_iff [UpwardEnumerable α]
-    [LinearlyUpwardEnumerable α] [InfinitelyUpwardEnumerable α] [SupportsUpperBound .open α]
-    [SupportsLowerBound .closed α] [LawfulUpwardEnumerableLowerBound .closed α]
-    [HasFiniteRanges .open α] [LawfulUpwardEnumerable α] [LawfulOpenUpperBound α]
-    {lower : Bound .closed α} {upper : Bound .open α} {a : α} :
-    (a ∈ (succ lower)...(succ upper)) ↔ ∃ a', a = succ a' ∧ a' ∈ lower...upper :=
-  mem_Rco_succ_succ_iff
+variable {α : Type u}
 
 private theorem eq_of_pairwise_lt_of_mem_iff_mem {lt : α → α → Prop} [asymm : Asymm lt]
     {l l' : List α} (hl : l.Pairwise lt) (hl' : l'.Pairwise lt)
@@ -268,55 +82,431 @@ private theorem eq_of_pairwise_lt_of_mem_iff_mem {lt : α → α → Prop} [asym
           have hgt := hl.1 y ‹_›
           cases Asymm.asymm _ _ hlt hgt
 
-public theorem toList_Rco_succ_succ_eq_map [UpwardEnumerable α] [SupportsLowerBound .closed α]
-    [LinearlyUpwardEnumerable α] [InfinitelyUpwardEnumerable α] [SupportsUpperBound .open α]
-    [HasFiniteRanges .open α] [LawfulUpwardEnumerable α] [LawfulOpenUpperBound α]
-    [LawfulUpwardEnumerableLowerBound .closed α] [LawfulUpwardEnumerableUpperBound .open α]
-    {lower : Bound .closed α} {upper : Bound .open α} :
-    ((succ lower)...(succ upper)).toList =
-      (lower...upper).toList.map succ := by
-  apply eq_of_pairwise_lt_of_mem_iff_mem (lt := UpwardEnumerable.LT) (asymm := ?_)
-  · apply pairwise_toList_upwardEnumerableLt
-  · apply List.Pairwise.map (R := UpwardEnumerable.LT) (S := UpwardEnumerable.LT)
-    · intro a b
-      exact UpwardEnumerable.succ_lt_succ_iff.mpr
-    · apply pairwise_toList_upwardEnumerableLt
-  · simp only [List.mem_map, mem_toList_iff_mem]
-    intro a
-    rw [mem_Rco_succ_succ_iff]
-    constructor
-    · rintro ⟨a, rfl, h⟩
-      exact ⟨a, h, rfl⟩
-    · rintro ⟨a, h, h'⟩
-      exact ⟨_, h'.symm, h⟩
-  · exact ⟨fun _ _ => UpwardEnumerable.not_gt_of_lt⟩
+theorem PRange.UpwardEnumerable.exists_of_succ_le [UpwardEnumerable α] [LawfulUpwardEnumerable α]
+    [InfinitelyUpwardEnumerable α]
+    {a b : α} (h : UpwardEnumerable.LE (succ a) b) :
+    ∃ b', b = succ b' ∧ UpwardEnumerable.LE a b' := by
+  obtain ⟨n, hn⟩ := h
+  rw [succMany?_eq_some_iff_succMany, succMany_succ_eq_succ_succMany] at hn
+  exact ⟨succMany n a, hn.symm, ⟨n, succMany?_eq_some⟩⟩
 
-@[deprecated toList_Rco_succ_succ_eq_map (since := "2025-08-22")]
-public theorem ClosedOpen.toList_succ_succ_eq_map [UpwardEnumerable α] [SupportsLowerBound .closed α]
-    [LinearlyUpwardEnumerable α] [InfinitelyUpwardEnumerable α] [SupportsUpperBound .open α]
-    [HasFiniteRanges .open α] [LawfulUpwardEnumerable α] [LawfulOpenUpperBound α]
-    [LawfulUpwardEnumerableLowerBound .closed α] [LawfulUpwardEnumerableUpperBound .open α]
-    {lower : Bound .closed α} {upper : Bound .open α} :
-    ((succ lower)...(succ upper)).toList =
-      (lower...upper).toList.map succ :=
-  toList_Rco_succ_succ_eq_map
-
-private theorem Internal.forIn'_eq_forIn'_iter [UpwardEnumerable α]
-    [SupportsUpperBound su α] [SupportsLowerBound sl α] [HasFiniteRanges su α]
-    [BoundedUpwardEnumerable sl α] [LawfulUpwardEnumerable α]
-    [LawfulUpwardEnumerableLowerBound sl α] [LawfulUpwardEnumerableUpperBound su α]
-    {r : PRange ⟨sl, su⟩ α}
-    {γ : Type u} {init : γ} {m : Type u → Type w} [Monad m] {f : (a : α) → a ∈ r → γ → m (ForInStep γ)} :
-    haveI := Iter.instForIn' (α := RangeIterator su α) (β := α) (n := m)
+private theorem Rcc.Internal.forIn'_eq_forIn'_iter [LE α] [DecidableLE α] [UpwardEnumerable α]
+    [LawfulUpwardEnumerableLE α] [Rxc.IsAlwaysFinite α] [LawfulUpwardEnumerable α]
+    {γ : Type u} {init : γ} {m : Type u → Type w} [Monad m] {r : Rcc α}
+    {f : (a : α) → a ∈ r → γ → m (ForInStep γ)} :
+    haveI := Iter.instForIn' (α := Rxc.Iterator α) (β := α) (n := m)
     ForIn'.forIn' r init f =
       ForIn'.forIn' (Internal.iter r) init (fun a ha acc => f a (Internal.isPlausibleIndirectOutput_iter_iff.mp ha) acc) := by
   rfl
 
-public theorem forIn'_eq_forIn'_toList [UpwardEnumerable α]
-    [SupportsUpperBound su α] [SupportsLowerBound sl α] [HasFiniteRanges su α]
-    [BoundedUpwardEnumerable sl α] [LawfulUpwardEnumerable α]
-    [LawfulUpwardEnumerableLowerBound sl α] [LawfulUpwardEnumerableUpperBound su α]
-    {r : PRange ⟨sl, su⟩ α}
+private theorem Rcc.Internal.toList_eq_toList_iter [LE α] [DecidableLE α]
+    [UpwardEnumerable α] [Rxc.IsAlwaysFinite α] [LawfulUpwardEnumerable α]
+    [LawfulUpwardEnumerableLE α] {r : Rcc α} :
+    r.toList = (Internal.iter r).toList := by
+  rfl
+
+private theorem Rco.Internal.forIn'_eq_forIn'_iter [LE α] [DecidableLE α] [LT α] [DecidableLT α]
+    [UpwardEnumerable α] [LawfulUpwardEnumerableLE α] [LawfulUpwardEnumerableLT α]
+    [Rxo.IsAlwaysFinite α] [LawfulUpwardEnumerable α]
+    {γ : Type u} {init : γ} {m : Type u → Type w} [Monad m] {r : Rco α}
+    {f : (a : α) → a ∈ r → γ → m (ForInStep γ)} :
+    haveI := Iter.instForIn' (α := Rxo.Iterator α) (β := α) (n := m)
+    ForIn'.forIn' r init f =
+      ForIn'.forIn' (Internal.iter r) init (fun a ha acc => f a (Internal.isPlausibleIndirectOutput_iter_iff.mp ha) acc) := by
+  rfl
+
+private theorem Rco.Internal.toList_eq_toList_iter [LE α] [LT α] [DecidableLT α]
+    [UpwardEnumerable α] [Rxo.IsAlwaysFinite α] [LawfulUpwardEnumerable α]
+    [LawfulUpwardEnumerableLT α] {r : Rco α} :
+    r.toList = (Internal.iter r).toList := by
+  rfl
+
+private theorem Rci.Internal.forIn'_eq_forIn'_iter [LE α] [DecidableLE α]
+    [UpwardEnumerable α] [LawfulUpwardEnumerableLE α]
+    [Rxi.IsAlwaysFinite α] [LawfulUpwardEnumerable α]
+    {γ : Type u} {init : γ} {m : Type u → Type w} [Monad m] {r : Rci α}
+    {f : (a : α) → a ∈ r → γ → m (ForInStep γ)} :
+    haveI := Iter.instForIn' (α := Rxi.Iterator α) (β := α) (n := m)
+    ForIn'.forIn' r init f =
+      ForIn'.forIn' (Internal.iter r) init (fun a ha acc => f a (Internal.isPlausibleIndirectOutput_iter_iff.mp ha) acc) := by
+  rfl
+
+private theorem Rci.Internal.toList_eq_toList_iter [LE α]
+    [UpwardEnumerable α] [Rxi.IsAlwaysFinite α] [LawfulUpwardEnumerable α] {r : Rci α} :
+    r.toList = (Internal.iter r).toList := by
+  rfl
+
+private theorem Roc.Internal.forIn'_eq_forIn'_iter [LE α] [DecidableLE α] [LT α] [DecidableLT α]
+    [UpwardEnumerable α] [LawfulUpwardEnumerableLE α] [LawfulUpwardEnumerableLT α]
+    [Rxc.IsAlwaysFinite α] [LawfulUpwardEnumerable α]
+    {γ : Type u} {init : γ} {m : Type u → Type w} [Monad m] {r : Roc α}
+    {f : (a : α) → a ∈ r → γ → m (ForInStep γ)} :
+    haveI := Iter.instForIn' (α := Rxc.Iterator α) (β := α) (n := m)
+    ForIn'.forIn' r init f =
+      ForIn'.forIn' (Internal.iter r) init (fun a ha acc => f a (Internal.isPlausibleIndirectOutput_iter_iff.mp ha) acc) := by
+  rfl
+
+private theorem Roc.Internal.toList_eq_toList_iter [LE α] [DecidableLE α]
+    [UpwardEnumerable α] [Rxc.IsAlwaysFinite α] [LawfulUpwardEnumerable α]
+    [LawfulUpwardEnumerableLE α] {r : Roc α} :
+    r.toList = (Internal.iter r).toList := by
+  rfl
+
+private theorem Roo.Internal.forIn'_eq_forIn'_iter [LT α] [DecidableLT α]
+    [UpwardEnumerable α] [LawfulUpwardEnumerableLT α] [Rxo.IsAlwaysFinite α]
+    [LawfulUpwardEnumerable α]
+    {γ : Type u} {init : γ} {m : Type u → Type w} [Monad m] {r : Roo α}
+    {f : (a : α) → a ∈ r → γ → m (ForInStep γ)} :
+    haveI := Iter.instForIn' (α := Rxo.Iterator α) (β := α) (n := m)
+    ForIn'.forIn' r init f =
+      ForIn'.forIn' (Internal.iter r) init (fun a ha acc => f a (Internal.isPlausibleIndirectOutput_iter_iff.mp ha) acc) := by
+  rfl
+
+private theorem Roo.Internal.toList_eq_toList_iter [LE α] [LT α] [DecidableLT α]
+    [UpwardEnumerable α] [Rxo.IsAlwaysFinite α] [LawfulUpwardEnumerable α]
+    [LawfulUpwardEnumerableLE α] {r : Roo α} :
+    r.toList = (Internal.iter r).toList := by
+  rfl
+
+private theorem Roi.Internal.forIn'_eq_forIn'_iter [LT α] [DecidableLT α]
+    [UpwardEnumerable α] [LawfulUpwardEnumerableLT α]
+    [Rxi.IsAlwaysFinite α] [LawfulUpwardEnumerable α]
+    {γ : Type u} {init : γ} {m : Type u → Type w} [Monad m] {r : Roi α}
+    {f : (a : α) → a ∈ r → γ → m (ForInStep γ)} :
+    haveI := Iter.instForIn' (α := Rxi.Iterator α) (β := α) (n := m)
+    ForIn'.forIn' r init f =
+      ForIn'.forIn' (Internal.iter r) init (fun a ha acc => f a (Internal.isPlausibleIndirectOutput_iter_iff.mp ha) acc) := by
+  rfl
+
+private theorem Roi.Internal.toList_eq_toList_iter [LE α]
+    [UpwardEnumerable α] [Rxi.IsAlwaysFinite α] [LawfulUpwardEnumerable α] {r : Roi α} :
+    r.toList = (Internal.iter r).toList := by
+  rfl
+
+public theorem Rxc.Iterator.toList_eq_match [LE α] [DecidableLE α]
+    [UpwardEnumerable α] [Rxc.IsAlwaysFinite α] [LawfulUpwardEnumerable α]
+    [LawfulUpwardEnumerableLE α]
+    {it : Iter (α := Rxc.Iterator α) α} :
+    it.toList =  match it.internalState.next with
+      | none => []
+      | some a => if a ≤ it.internalState.upperBound then
+          a :: (⟨⟨UpwardEnumerable.succ? a, it.internalState.upperBound⟩⟩ : Iter (α := Rxc.Iterator α) α).toList
+        else
+          [] := by
+  apply Eq.symm
+  rw [Iter.toList_eq_match_step, Rxc.Iterator.step_eq_step]
+  simp only [Rxc.Iterator.step]
+  split <;> rename_i heq
+  · simp [*]
+  · split <;> rename_i heq' <;> simp [*]
+
+public theorem Rxo.Iterator.toList_eq_match [LT α] [DecidableLT α]
+    [UpwardEnumerable α] [Rxo.IsAlwaysFinite α] [LawfulUpwardEnumerable α]
+    [LawfulUpwardEnumerableLT α]
+    {it : Iter (α := Rxo.Iterator α) α} :
+    it.toList =  match it.internalState.next with
+      | none => []
+      | some a => if a < it.internalState.upperBound then
+          a :: (⟨⟨UpwardEnumerable.succ? a, it.internalState.upperBound⟩⟩ : Iter (α := Rxo.Iterator α) α).toList
+        else
+          [] := by
+  apply Eq.symm
+  simp only [Iter.toList_eq_match_step (it := it), Rxo.Iterator.step_eq_step, Rxo.Iterator.step]
+  split <;> rename_i heq
+  · simp [*]
+  · split <;> rename_i heq' <;> simp [*]
+
+public theorem Rxi.Iterator.toList_eq_match
+    [UpwardEnumerable α] [Rxi.IsAlwaysFinite α] [LawfulUpwardEnumerable α]
+    {it : Iter (α := Rxi.Iterator α) α} :
+    it.toList =  match it.internalState.next with
+      | none => []
+      | some a =>
+          a :: (⟨⟨UpwardEnumerable.succ? a⟩⟩ : Iter (α := Rxi.Iterator α) α).toList := by
+  apply Eq.symm
+  simp only [Iter.toList_eq_match_step (it := it), Rxi.Iterator.step_eq_step, Rxi.Iterator.step]
+  split <;> rename_i heq <;> simp [*]
+
+public theorem Rxc.Iterator.pairwise_toList_upwardEnumerableLt [LE α] [DecidableLE α]
+    [UpwardEnumerable α] [LawfulUpwardEnumerable α] [LawfulUpwardEnumerableLE α]
+    [Rxc.IsAlwaysFinite α] [LawfulUpwardEnumerable α]
+    (it : Iter (α := Rxc.Iterator α) α) :
+    it.toList.Pairwise (fun a b => UpwardEnumerable.LT a b) := by
+  induction it using Iter.inductSteps with | step it ihy ihs
+  rw [Rxc.Iterator.toList_eq_match]
+  repeat' split <;> (try exact .nil; done)
+  rename_i a _ _
+  apply List.Pairwise.cons
+  · intro a' ha
+    rw [Iter.mem_toList_iff_isPlausibleIndirectOutput] at ha
+    replace ha := Rxc.Iterator.upwardEnumerableLe_of_isPlausibleIndirectOutput ha
+    simp only at ha
+    have : UpwardEnumerable.LT a ha.choose := by
+      refine ⟨0, ?_⟩
+      simp only [succMany?_succ?, succMany?_zero,
+        Option.bind_some]
+      exact ha.choose_spec.1
+    exact UpwardEnumerable.lt_of_lt_of_le this ha.choose_spec.2
+  · apply ihy (out := a)
+    simp_all [Rxc.Iterator.isPlausibleStep_iff, Rxc.Iterator.step]
+
+public theorem Rxo.Iterator.pairwise_toList_upwardEnumerableLt [LT α] [DecidableLT α]
+    [UpwardEnumerable α] [LawfulUpwardEnumerable α] [LawfulUpwardEnumerableLT α]
+    [Rxo.IsAlwaysFinite α] [LawfulUpwardEnumerable α]
+    (it : Iter (α := Rxo.Iterator α) α) :
+    it.toList.Pairwise (fun a b => UpwardEnumerable.LT a b) := by
+  induction it using Iter.inductSteps with | step it ihy ihs
+  rw [Rxo.Iterator.toList_eq_match]
+  repeat' split <;> (try exact .nil; done)
+  rename_i a _ _
+  apply List.Pairwise.cons
+  · intro a' ha
+    rw [Iter.mem_toList_iff_isPlausibleIndirectOutput] at ha
+    replace ha := Rxo.Iterator.upwardEnumerableLe_of_isPlausibleIndirectOutput ha
+    simp only at ha
+    have : UpwardEnumerable.LT a ha.choose := by
+      refine ⟨0, ?_⟩
+      simp only [succMany?_succ?, succMany?_zero,
+        Option.bind_some]
+      exact ha.choose_spec.1
+    exact UpwardEnumerable.lt_of_lt_of_le this ha.choose_spec.2
+  · apply ihy (out := a)
+    simp_all [Rxo.Iterator.isPlausibleStep_iff, Rxo.Iterator.step]
+
+public theorem Rxi.Iterator.pairwise_toList_upwardEnumerableLt
+    [UpwardEnumerable α] [LawfulUpwardEnumerable α]
+    [Rxi.IsAlwaysFinite α] [LawfulUpwardEnumerable α]
+    (it : Iter (α := Rxi.Iterator α) α) :
+    it.toList.Pairwise (fun a b => UpwardEnumerable.LT a b) := by
+  induction it using Iter.inductSteps with | step it ihy ihs
+  rw [Rxi.Iterator.toList_eq_match]
+  repeat' split <;> (try exact .nil; done)
+  rename_i a _
+  apply List.Pairwise.cons
+  · intro a' ha
+    rw [Iter.mem_toList_iff_isPlausibleIndirectOutput] at ha
+    replace ha := Rxi.Iterator.upwardEnumerableLe_of_isPlausibleIndirectOutput ha
+    simp only at ha
+    have : UpwardEnumerable.LT a ha.choose := by
+      refine ⟨0, ?_⟩
+      simp only [succMany?_succ?, succMany?_zero,
+        Option.bind_some]
+      exact ha.choose_spec.1
+    exact UpwardEnumerable.lt_of_lt_of_le this ha.choose_spec.2
+  · apply ihy (out := a)
+    simp_all [Rxi.Iterator.isPlausibleStep_iff, Rxi.Iterator.step]
+
+public instance [LE α] [DecidableLE α] [UpwardEnumerable α] [Rxc.HasSize α] [Rxc.LawfulHasSize α]
+    [LawfulUpwardEnumerableLE α] [Rxc.IsAlwaysFinite α] [LawfulUpwardEnumerable α] :
+    LawfulIteratorSize (Rxc.Iterator α) where
+  size_eq_size_toArray {it} := by
+    simp only [Iter.size, IteratorSize.size, Iter.toIterM]
+    split <;> rename_i heq
+    · simp [Iter.toArray_eq_match_step (it := it), Rxc.Iterator.step_eq_step, Rxc.Iterator.step, heq]
+    · rename_i next
+      simp only [Id.run_pure]
+      induction h : Rxc.HasSize.size _ it.internalState.upperBound generalizing it next
+      · simp only [Rxc.size_eq_zero_iff_not_le] at h
+        simp [Iter.toArray_eq_match_step (it := it), Rxc.Iterator.step_eq_step, Rxc.Iterator.step, heq, h]
+      · rename_i ih
+        have h' : next ≤ it.internalState.upperBound := Rxc.size_pos_iff_isSatisfied.mp (by omega)
+        simp only [Iter.toArray_eq_match_step (it := it), Rxc.Iterator.step_eq_step,
+            Rxc.Iterator.step, heq, h', ↓reduceIte]
+        cases hn : UpwardEnumerable.succ? next
+        · rw [Iter.toArray_eq_match_step, Rxc.Iterator.step_eq_step]
+          simp_all [Rxc.Iterator.step, Rxc.LawfulHasSize.size_eq_one_of_succ?_eq_none _ _ h' hn]
+        · have := Rxc.LawfulHasSize.size_eq_succ_of_succ?_eq_some _ _ _ h' hn
+          simp only [Array.size_append, List.size_toArray, List.length_cons, List.length_nil,
+            Nat.zero_add]
+          rw [← ih _ rfl] <;> (try simp) <;> omega
+
+public instance [LT α] [DecidableLT α] [UpwardEnumerable α] [Rxo.HasSize α]
+    [Rxo.LawfulHasSize α] [LawfulUpwardEnumerableLT α] [Rxo.IsAlwaysFinite α]
+    [LawfulUpwardEnumerable α] :
+    LawfulIteratorSize (Rxo.Iterator α) where
+  size_eq_size_toArray {it} := by
+    simp only [Iter.size, IteratorSize.size, Iter.toIterM]
+    split <;> rename_i heq
+    · simp [Iter.toArray_eq_match_step (it := it), Rxo.Iterator.step_eq_step, Rxo.Iterator.step, heq]
+    · rename_i next
+      simp only [Id.run_pure]
+      induction h : Rxo.HasSize.size _ it.internalState.upperBound generalizing it next
+      · simp only [Rxo.size_eq_zero_iff_not_le] at h
+        simp [Iter.toArray_eq_match_step (it := it), Rxo.Iterator.step_eq_step, Rxo.Iterator.step, heq, h]
+      · rename_i ih
+        have h' : next < it.internalState.upperBound := Rxo.size_pos_iff_isSatisfied.mp (by omega)
+        simp only [Iter.toArray_eq_match_step (it := it), Rxo.Iterator.step_eq_step,
+            Rxo.Iterator.step, heq, h', ↓reduceIte]
+        cases hn : UpwardEnumerable.succ? next
+        · rw [Iter.toArray_eq_match_step, Rxo.Iterator.step_eq_step]
+          simp_all [Rxo.Iterator.step, Rxo.LawfulHasSize.size_eq_one_of_succ?_eq_none _ _ h' hn]
+        · have := Rxo.LawfulHasSize.size_eq_succ_of_succ?_eq_some _ _ _ h' hn
+          simp only [Array.size_append, List.size_toArray, List.length_cons, List.length_nil,
+            Nat.zero_add]
+          rw [← ih _ rfl] <;> (try simp) <;> omega
+
+namespace Rcc
+
+variable {r : Rcc α}
+
+public theorem toList_eq_match [LE α] [DecidableLE α] [UpwardEnumerable α]
+    [LawfulUpwardEnumerable α] [LawfulUpwardEnumerableLE α] [Rxc.IsAlwaysFinite α]
+    [LawfulUpwardEnumerable α] :
+    r.toList = if r.lower ≤ r.upper then
+        r.lower :: (r.lower<...=r.upper).toList
+      else
+        [] := by
+  rw [Internal.toList_eq_toList_iter, Rxc.Iterator.toList_eq_match]; rfl
+
+public theorem toList_eq_nil_iff [LE α] [DecidableLE α] [UpwardEnumerable α]
+    [LawfulUpwardEnumerable α] [LawfulUpwardEnumerableLE α] [Rxc.IsAlwaysFinite α]
+    [LawfulUpwardEnumerable α] :
+    r.toList = [] ↔ ¬ (r.lower ≤ r.upper) := by
+  rw [Internal.toList_eq_toList_iter, Rxc.Iterator.toList_eq_match, Internal.iter]
+  simp only
+  split <;> rename_i heq <;> simp [heq]
+
+public theorem mem_toList_iff_mem [LE α] [DecidableLE α] [UpwardEnumerable α]
+    [LawfulUpwardEnumerable α] [LawfulUpwardEnumerableLE α] [Rxc.IsAlwaysFinite α]
+    [LawfulUpwardEnumerable α] {a : α} : a ∈ r.toList ↔ a ∈ r := by
+  rw [Internal.toList_eq_toList_iter, Iter.mem_toList_iff_isPlausibleIndirectOutput,
+    Internal.isPlausibleIndirectOutput_iter_iff]
+
+-- public theorem BoundedUpwardEnumerable.init?_succ?_closed [UpwardEnumerable α]
+--     [LawfulUpwardEnumerable α] {lower lower' : Bound .closed α}
+--     (h : UpwardEnumerable.succ? lower = some lower') :
+--     init? lower' = (init? lower).bind UpwardEnumerable.succ? := by
+--   cases h : init? lower <;> rename_i ilower <;> cases h' : init? lower' <;> rename_i ilower'
+--   · simp
+--   · simp [init?] at h
+--   · simp [init?] at h'
+--   · simp_all [init?]
+
+-- @[deprecated BoundedUpwardEnumerable.init?_succ?_closed (since := "2025-08-22")]
+-- public theorem BoundedUpwardEnumerable.Closed.init?_succ [UpwardEnumerable α]
+--     [LawfulUpwardEnumerable α] {lower lower' : Bound .closed α}
+--     (h : UpwardEnumerable.succ? lower = some lower') :
+--     init? lower' = (init? lower).bind UpwardEnumerable.succ? :=
+--   init?_succ?_closed h
+
+public theorem pairwise_toList_upwardEnumerableLt [LE α] [DecidableLE α]
+    [UpwardEnumerable α] [LawfulUpwardEnumerable α] [LawfulUpwardEnumerableLE α]
+    [Rxc.IsAlwaysFinite α] [LawfulUpwardEnumerable α] :
+    r.toList.Pairwise (fun a b => UpwardEnumerable.LT a b) := by
+  rw [Internal.toList_eq_toList_iter]
+  apply Rxc.Iterator.pairwise_toList_upwardEnumerableLt
+
+public theorem pairwise_toList_ne [LE α] [DecidableLE α]
+    [UpwardEnumerable α] [LawfulUpwardEnumerable α] [LawfulUpwardEnumerableLE α]
+    [Rxc.IsAlwaysFinite α] [LawfulUpwardEnumerable α] :
+    r.toList.Pairwise (fun a b => a ≠ b) :=
+  List.Pairwise.imp (fun hlt => UpwardEnumerable.ne_of_lt hlt) pairwise_toList_upwardEnumerableLt
+
+public theorem pairwise_toList_lt [LE α] [DecidableLE α] [LT α]
+    [UpwardEnumerable α] [LawfulUpwardEnumerable α] [LawfulUpwardEnumerableLE α]
+    [LawfulUpwardEnumerableLT α] [Rxc.IsAlwaysFinite α] [LawfulUpwardEnumerable α] :
+    r.toList.Pairwise (fun a b => a < b) :=
+  List.Pairwise.imp
+    (fun hlt => (LawfulUpwardEnumerableLT.lt_iff ..).mpr hlt) pairwise_toList_upwardEnumerableLt
+
+public theorem pairwise_toList_le [LE α] [DecidableLE α] [LT α]
+    [UpwardEnumerable α] [LawfulUpwardEnumerable α] [LawfulUpwardEnumerableLE α]
+    [Rxc.IsAlwaysFinite α] [LawfulUpwardEnumerable α] :
+    r.toList.Pairwise (fun a b => a ≤ b) :=
+  pairwise_toList_upwardEnumerableLt
+    |> List.Pairwise.imp UpwardEnumerable.le_of_lt
+    |> List.Pairwise.imp (fun hle => (UpwardEnumerable.le_iff ..).mpr hle)
+
+-- public theorem mem_Rco_succ_succ_iff [LE α] [DecidableLE α] [UpwardEnumerable α]
+--     [LinearlyUpwardEnumerable α] [LawfulUpwardEnumerableLE α] [InfinitelyUpwardEnumerable α]
+--     [HasFiniteRanges .open α] [LawfulUpwardEnumerable α] [LawfulOpenUpperBound α]
+--     {lower : Bound .closed α} {upper : Bound .open α} {a : α} :
+--     (a ∈ (succ lower)...(succ upper)) ↔ ∃ a', a = succ a' ∧ a' ∈ lower...upper := by
+--   simp [Membership.mem, LawfulUpwardEnumerableLowerBound.isSatisfied_iff,
+--     init?, LawfulOpenUpperBound.isSatisfied_iff_le]
+--   rw [← Option.some_get (InfinitelyUpwardEnumerable.isSome_succ? _)]
+--   simp only [Option.some.injEq, ← UpwardEnumerable.succ.eq_def]
+--   simp
+--   constructor
+--   · rintro ⟨⟨n, hn⟩, h⟩
+--     rw [succMany?_eq_some_iff_succMany, ← succMany_one, ← succMany_add, Nat.add_comm, succMany_add,
+--       succMany_one] at hn
+--     rw [← hn]
+--     refine ⟨succMany n lower, rfl, ?_, ?_⟩
+--     · exact ⟨n, by simp [succMany_eq_get]⟩
+--     · obtain ⟨m, hm⟩ := h
+--       refine ⟨m, ?_⟩
+--       rw [succMany?_eq_some_iff_succMany] at hm ⊢
+--       rwa [← hn, ← succMany_one, ← succMany_add, Nat.add_comm, succMany_add, succMany_one,
+--         succ_eq_succ_iff] at hm
+--   · rintro ⟨a', rfl, hl, hu⟩
+--     simp [UpwardEnumerable.succ_le_succ_iff, UpwardEnumerable.succ_lt_succ_iff]
+--     exact ⟨hl, hu⟩
+
+public theorem mem_succ_succ_iff [LE α] [DecidableLE α] [UpwardEnumerable α]
+    [LinearlyUpwardEnumerable α] [LawfulUpwardEnumerableLE α] [InfinitelyUpwardEnumerable α]
+    [Rxc.IsAlwaysFinite α] [LawfulUpwardEnumerable α] {lo hi a : α} :
+    (a ∈ (succ lo)...=(succ hi)) ↔ ∃ a', a = succ a' ∧ a' ∈ lo...=hi := by
+  simp [Membership.mem, LawfulUpwardEnumerableLE.le_iff]
+  constructor
+  · intro h
+    obtain ⟨a', rfl, ha'⟩ := UpwardEnumerable.exists_of_succ_le h.1
+    exact ⟨a', rfl, ha', UpwardEnumerable.succ_le_succ_iff.mp h.2⟩
+  · rintro ⟨a', rfl, hl, hu⟩
+    simp only [UpwardEnumerable.succ_le_succ_iff]
+    exact ⟨hl, hu⟩
+
+public theorem succ_mem_succ_succ_iff [LE α] [DecidableLE α] [UpwardEnumerable α]
+    [LinearlyUpwardEnumerable α] [LawfulUpwardEnumerableLE α] [InfinitelyUpwardEnumerable α]
+    [Rxc.IsAlwaysFinite α] [LawfulUpwardEnumerable α] {lo hi a : α} :
+    (succ a ∈ (succ lo)...=(succ hi)) ↔ a ∈ lo...=hi := by
+  simp [mem_succ_succ_iff, UpwardEnumerable.succ_inj]
+
+-- public theorem toList_Rco_succ_succ_eq_map [UpwardEnumerable α] [SupportsLowerBound .closed α]
+--     [LinearlyUpwardEnumerable α] [InfinitelyUpwardEnumerable α] [SupportsUpperBound .open α]
+--     [HasFiniteRanges .open α] [LawfulUpwardEnumerable α] [LawfulOpenUpperBound α]
+--     [LawfulUpwardEnumerableLowerBound .closed α] [LawfulUpwardEnumerableUpperBound .open α]
+--     {lower : Bound .closed α} {upper : Bound .open α} :
+--     ((succ lower)...(succ upper)).toList =
+--       (lower...upper).toList.map succ := by
+--   apply eq_of_pairwise_lt_of_mem_iff_mem (lt := UpwardEnumerable.LT) (asymm := ?_)
+--   · apply pairwise_toList_upwardEnumerableLt
+--   · apply List.Pairwise.map (R := UpwardEnumerable.LT) (S := UpwardEnumerable.LT)
+--     · intro a b
+--       exact UpwardEnumerable.succ_lt_succ_iff.mpr
+--     · apply pairwise_toList_upwardEnumerableLt
+--   · simp only [List.mem_map, mem_toList_iff_mem]
+--     intro a
+--     rw [mem_Rco_succ_succ_iff]
+--     constructor
+--     · rintro ⟨a, rfl, h⟩
+--       exact ⟨a, h, rfl⟩
+--     · rintro ⟨a, h, h'⟩
+--       exact ⟨_, h'.symm, h⟩
+--   · exact ⟨fun _ _ => UpwardEnumerable.not_gt_of_lt⟩
+
+public theorem toList_succ_succ_eq_map [LE α] [DecidableLE α] [UpwardEnumerable α]
+    [LinearlyUpwardEnumerable α] [LawfulUpwardEnumerableLE α] [InfinitelyUpwardEnumerable α]
+    [Rxc.IsAlwaysFinite α] [LawfulUpwardEnumerable α] {lo hi : α} :
+    ((succ lo)...=(succ hi)).toList =
+      (lo...=hi).toList.map succ := by
+  apply eq_of_pairwise_lt_of_mem_iff_mem (lt := UpwardEnumerable.LT)
+  · exact pairwise_toList_upwardEnumerableLt
+  · apply List.Pairwise.map (R := UpwardEnumerable.LT) (S := UpwardEnumerable.LT)
+    · exact fun _ _ => UpwardEnumerable.succ_lt_succ_iff.mpr
+    · exact pairwise_toList_upwardEnumerableLt
+  · simp [List.mem_map, mem_toList_iff_mem, mem_succ_succ_iff, eq_comm, and_comm]
+
+@[deprecated Rcc.toList_succ_succ_eq_map (since := "2025-08-22")]
+public theorem ClosedOpen.toList_succ_succ_eq_map [LE α] [DecidableLE α] [UpwardEnumerable α]
+    [LinearlyUpwardEnumerable α] [LawfulUpwardEnumerableLE α] [InfinitelyUpwardEnumerable α]
+    [Rxc.IsAlwaysFinite α] [LawfulUpwardEnumerable α] {lo hi : α} :
+    ((succ lo)...=(succ hi)).toList =
+      (lo...=hi).toList.map succ :=
+  Rcc.toList_succ_succ_eq_map
+
+public theorem forIn'_eq_forIn'_toList [LE α] [DecidableLE α] [UpwardEnumerable α]
+    [LawfulUpwardEnumerableLE α] [Rxc.IsAlwaysFinite α] [LawfulUpwardEnumerable α]
     {γ : Type u} {init : γ} {m : Type u → Type w} [Monad m] [LawfulMonad m]
     {f : (a : α) → a ∈ r → γ → m (ForInStep γ)} :
     ForIn'.forIn' r init f =
@@ -324,135 +514,555 @@ public theorem forIn'_eq_forIn'_toList [UpwardEnumerable α]
   simp [Internal.forIn'_eq_forIn'_iter, Internal.toList_eq_toList_iter,
     Iter.forIn'_eq_forIn'_toList]
 
-public theorem forIn'_toList_eq_forIn' [UpwardEnumerable α]
-    [SupportsUpperBound su α] [SupportsLowerBound sl α] [HasFiniteRanges su α]
-    [BoundedUpwardEnumerable sl α] [LawfulUpwardEnumerable α]
-    [LawfulUpwardEnumerableLowerBound sl α] [LawfulUpwardEnumerableUpperBound su α]
-    {r : PRange ⟨sl, su⟩ α}
+public theorem forIn'_toList_eq_forIn' [LE α] [DecidableLE α] [UpwardEnumerable α]
+    [LawfulUpwardEnumerableLE α] [Rxc.IsAlwaysFinite α] [LawfulUpwardEnumerable α]
     {γ : Type u} {init : γ} {m : Type u → Type w} [Monad m] [LawfulMonad m]
     {f : (a : α) → _ → γ → m (ForInStep γ)} :
     ForIn'.forIn' r.toList init f =
       ForIn'.forIn' r init (fun a ha acc => f a (mem_toList_iff_mem.mpr ha) acc) := by
   simp [forIn'_eq_forIn'_toList]
 
-public theorem mem_of_mem_open [UpwardEnumerable α]
-    [SupportsUpperBound su α] [SupportsLowerBound sl α] [HasFiniteRanges su α]
-    [BoundedUpwardEnumerable sl α] [LawfulUpwardEnumerable α]
-    [LawfulUpwardEnumerableLowerBound sl α] [LawfulUpwardEnumerableUpperBound su α]
-    [SupportsLowerBound .open α] [LawfulUpwardEnumerableLowerBound .open α]
-    {r : PRange ⟨sl, su⟩ α} {a b : α}
-    (hrb : SupportsLowerBound.IsSatisfied r.lower b)
-    (hmem : a ∈ PRange.mk (shape := ⟨.open, su⟩) b r.upper) :
+public theorem mem_of_mem_Roc [LE α] [LT α] [UpwardEnumerable α]
+    [LawfulUpwardEnumerableLE α] [LawfulUpwardEnumerableLT α] [Rxc.IsAlwaysFinite α]
+    [LawfulUpwardEnumerable α] {a b : α}
+    (hrb : r.lower ≤ b)
+    (hmem : a ∈ b<...=r.upper) :
     a ∈ r := by
-  refine ⟨?_, hmem.2⟩
-  have := hmem.1
-  simp only [LawfulUpwardEnumerableLowerBound.isSatisfied_iff, init?] at this hrb ⊢
-  obtain ⟨init, hi⟩ := hrb
-  obtain ⟨b', hb'⟩ := this
-  refine ⟨init, hi.1, UpwardEnumerable.le_trans hi.2 (UpwardEnumerable.le_trans ?_ hb'.2)⟩
-  exact UpwardEnumerable.le_of_succ?_eq hb'.1
+  haveI := UpwardEnumerable.instLETransOfLawfulUpwardEnumerableLE (α := α)
+  refine ⟨le_trans hrb ?_, hmem.2⟩
+  simp only [Membership.mem, LawfulUpwardEnumerableLE.le_iff, LawfulUpwardEnumerableLT.lt_iff] at hmem ⊢
+  exact UpwardEnumerable.le_of_lt hmem.1
 
-public theorem SupportsLowerBound.isSatisfied_init? {sl} [UpwardEnumerable α]
-    [SupportsLowerBound sl α] [BoundedUpwardEnumerable sl α] [LawfulUpwardEnumerable α]
-    [LawfulUpwardEnumerableLowerBound sl α]
-    {bound : Bound sl α} {a : α} (h : init? bound = some a) :
-    SupportsLowerBound.IsSatisfied bound a := by
-  simp only [LawfulUpwardEnumerableLowerBound.isSatisfied_iff]
-  exact ⟨a, h, UpwardEnumerable.le_refl _⟩
+-- public theorem SupportsLowerBound.isSatisfied_init? {sl} [UpwardEnumerable α]
+--     [SupportsLowerBound sl α] [BoundedUpwardEnumerable sl α] [LawfulUpwardEnumerable α]
+--     [LawfulUpwardEnumerableLowerBound sl α]
+--     {bound : Bound sl α} {a : α} (h : init? bound = some a) :
+--     SupportsLowerBound.IsSatisfied bound a := by
+--   simp only [LawfulUpwardEnumerableLowerBound.isSatisfied_iff]
+--   exact ⟨a, h, UpwardEnumerable.le_refl _⟩
 
-public theorem forIn'_eq_match {sl su} [UpwardEnumerable α]
-    [SupportsUpperBound su α] [SupportsLowerBound sl α] [HasFiniteRanges su α]
-    [BoundedUpwardEnumerable sl α] [LawfulUpwardEnumerable α]
-    [LawfulUpwardEnumerableLowerBound sl α] [LawfulUpwardEnumerableUpperBound su α]
-    [SupportsLowerBound .open α] [LawfulUpwardEnumerableLowerBound .open α]
-    {r : PRange ⟨sl, su⟩ α}
-    {γ : Type u} {init : γ} {m : Type u → Type w} [Monad m] [LawfulMonad m]
-    {f : (a : α) → _ → γ → m (ForInStep γ)} :
-    ForIn'.forIn' r init f = match hi : init? r.lower with
-      | none => pure init
-      | some a => if hu : SupportsUpperBound.IsSatisfied r.upper a then do
-        match ← f a ⟨SupportsLowerBound.isSatisfied_init? hi, hu⟩ init with
+public theorem forIn'_eq_match_Roc [LE α] [DecidableLE α] [LT α] [DecidableLT α]
+    [UpwardEnumerable α] [LawfulUpwardEnumerableLT α] [LawfulUpwardEnumerableLE α]
+    [Rxc.IsAlwaysFinite α] [LawfulUpwardEnumerable α]
+    {m : Type u → Type w} [Monad m] [LawfulMonad m]
+    {γ : Type u} {init : γ} {f : (a : α) → _ → γ → m (ForInStep γ)} :
+    ForIn'.forIn' r init f = if hu : r.lower ≤ r.upper then do
+        have hle : r.lower ≤ r.lower := by
+          simpa [UpwardEnumerable.le_iff] using UpwardEnumerable.le_refl _
+        match ← f r.lower ⟨hle, hu⟩ init with
         | .yield c =>
-          ForIn'.forIn' (α := α) (β := γ) (PRange.mk (shape := ⟨.open, su⟩) a r.upper) c
-            (fun a ha acc => f a (mem_of_mem_open (SupportsLowerBound.isSatisfied_init? hi) ha) acc)
+          ForIn'.forIn' (α := α) (β := γ) (r.lower<...=r.upper) c
+            (fun a ha acc => f a (mem_of_mem_Roc hle ha) acc)
         | .done c => return c
       else
         return init := by
-  rw [Internal.forIn'_eq_forIn'_iter, Iter.forIn'_eq_match_step]
-  simp only [RangeIterator.step_eq_step, RangeIterator.step, Internal.iter]
   apply Eq.symm
-  split <;> rename_i heq
-  · simp [heq]
-  · simp only [heq]
-    split
-    · simp only
-      apply bind_congr
-      intro step
-      split
-      · simp [Internal.forIn'_eq_forIn'_iter, Internal.iter, BoundedUpwardEnumerable.init?]
-      · simp
-    · simp
+  rw [Internal.forIn'_eq_forIn'_iter, Iter.forIn'_eq_match_step]
+  simp only [Rxc.Iterator.step_eq_step, Rxc.Iterator.step, Internal.iter]
+  split
+  · apply bind_congr; intro step
+    split <;> simp [Roc.Internal.forIn'_eq_forIn'_iter, Roc.Internal.iter]
+  · simp
 
-public instance {su} [UpwardEnumerable α] [SupportsUpperBound su α] [RangeSize su α]
-    [LawfulUpwardEnumerable α] [HasFiniteRanges su α] [LawfulRangeSize su α] :
-    LawfulIteratorSize (RangeIterator su α) where
-  size_eq_size_toArray {it} := by
-    simp only [Iter.size, IteratorSize.size, Iter.toIterM]
-    split <;> rename_i heq
-    · rw [Iter.toArray_eq_match_step, RangeIterator.step_eq_step]
-      simp [RangeIterator.step, heq]
-    · rename_i next
-      simp only [Id.run_pure]
-      induction h : RangeSize.size it.internalState.upperBound _ generalizing it next
-      · rw [Iter.toArray_eq_match_step, RangeIterator.step_eq_step]
-        simp only [RangeIterator.step, heq]
-        by_cases h : SupportsUpperBound.IsSatisfied it.internalState.upperBound next
-        · exfalso
-          cases hn : UpwardEnumerable.succ? next
-          · have := LawfulRangeSize.size_eq_one_of_succ?_eq_none _ _ h hn
-            simp [*] at this
-          · have := LawfulRangeSize.size_eq_succ_of_succ?_eq_some _ _ _ h hn
-            simp [*] at this
-        · simp [h]
-      · rename_i ih
-        by_cases h' : SupportsUpperBound.IsSatisfied it.internalState.upperBound next
-        · rw [Iter.toArray_eq_match_step, RangeIterator.step_eq_step]
-          simp only [RangeIterator.step, heq, h', ↓reduceIte, Array.size_append, List.size_toArray,
-            List.length_cons, List.length_nil, Nat.zero_add]
-          cases hn : UpwardEnumerable.succ? next
-          · rw [Iter.toArray_eq_match_step, RangeIterator.step_eq_step]
-            simp only [RangeIterator.step, Array.size_empty]
-            simp_all [LawfulRangeSize.size_eq_one_of_succ?_eq_none _ _ h' hn]
-          · rename_i next'
-            have := LawfulRangeSize.size_eq_succ_of_succ?_eq_some _ _ _ h' hn
-            simp only [this, Nat.add_right_cancel_iff] at h
-            specialize ih (it := ⟨⟨some next', it.internalState.upperBound⟩⟩) next' rfl h
-            rw [ih, Nat.add_comm]
-        · have := LawfulRangeSize.size_eq_zero_of_not_isSatisfied _ _ h'
-          simp [*] at this
-
-public theorem isEmpty_iff_forall_not_mem {sl su} [UpwardEnumerable α] [LawfulUpwardEnumerable α]
-    [BoundedUpwardEnumerable sl α] [SupportsLowerBound sl α] [SupportsUpperBound su α]
-    [LawfulUpwardEnumerableLowerBound sl α] [LawfulUpwardEnumerableUpperBound su α]
-    {r : PRange ⟨sl, su⟩ α} :
+public theorem isEmpty_iff_forall_not_mem [LE α] [DecidableLE α] [UpwardEnumerable α]
+    [Rxc.HasSize α] [Rxc.LawfulHasSize α] [LawfulUpwardEnumerableLE α] [Rxc.IsAlwaysFinite α]
+    [LawfulUpwardEnumerable α] :
     r.isEmpty ↔ ∀ a, ¬ a ∈ r := by
-  simp only [PRange.isEmpty, Option.all_eq_true_iff_get]
+  simp only [isEmpty, decide_eq_true_eq]
   constructor
-  · intro h a hmem
-    have hl := hmem.1
-    have hu := hmem.2
-    simp only [LawfulUpwardEnumerableLowerBound.isSatisfied_iff] at hl
-    obtain ⟨init, hi, hl⟩ := hl
-    have : SupportsUpperBound.IsSatisfied r.upper init :=
-      LawfulUpwardEnumerableUpperBound.isSatisfied_of_le r.upper _ a hu hl
-    simp only [Option.eq_some_iff_get_eq] at hi
-    specialize h hi.choose
-    simp [hi.choose_spec, this] at h
+  · rintro h a ⟨hl, hu⟩
+    simp only [UpwardEnumerable.le_iff] at h hl hu
+    exact h.elim (UpwardEnumerable.le_trans hl hu)
   · intro h hi
-    simp only [Bool.not_eq_eq_eq_not, Bool.not_true, decide_eq_false_iff_not]
-    intro hu
-    have hl := SupportsLowerBound.isSatisfied_init? (bound := r.lower)
-      (Option.some_get hi).symm
-    exact h ((init? r.lower).get hi) ⟨hl, hu⟩
+    refine h r.lower ⟨?_, hi⟩
+    simpa [UpwardEnumerable.le_iff] using UpwardEnumerable.le_refl _
 
-end Std.PRange
+end Rcc
+
+namespace Rco
+
+variable {r : Rco α}
+
+public theorem toList_eq_match [LE α] [LT α] [DecidableLT α] [UpwardEnumerable α]
+    [LawfulUpwardEnumerable α] [LawfulUpwardEnumerableLT α] [Rxo.IsAlwaysFinite α]
+    [LawfulUpwardEnumerable α] :
+    r.toList = if r.lower < r.upper then
+        r.lower :: (r.lower<...<r.upper).toList
+      else
+        [] := by
+  rw [Internal.toList_eq_toList_iter, Rxo.Iterator.toList_eq_match]; rfl
+
+public theorem toList_eq_nil_iff [LE α] [LT α] [DecidableLT α] [UpwardEnumerable α]
+    [LawfulUpwardEnumerable α] [LawfulUpwardEnumerableLT α] [Rxo.IsAlwaysFinite α]
+    [LawfulUpwardEnumerable α] :
+    r.toList = [] ↔ ¬ (r.lower < r.upper) := by
+  rw [Internal.toList_eq_toList_iter, Rxo.Iterator.toList_eq_match, Internal.iter]
+  simp only
+  split <;> rename_i heq <;> simp [heq]
+
+public theorem mem_toList_iff_mem [LE α] [DecidableLE α] [LT α] [DecidableLT α] [UpwardEnumerable α]
+    [LawfulUpwardEnumerable α] [LawfulUpwardEnumerableLT α] [LawfulUpwardEnumerableLE α]
+    [Rxo.IsAlwaysFinite α] [LawfulUpwardEnumerable α] {a : α} : a ∈ r.toList ↔ a ∈ r := by
+  rw [Internal.toList_eq_toList_iter, Iter.mem_toList_iff_isPlausibleIndirectOutput,
+    Internal.isPlausibleIndirectOutput_iter_iff]
+
+-- public theorem BoundedUpwardEnumerable.init?_succ?_closed [UpwardEnumerable α]
+--     [LawfulUpwardEnumerable α] {lower lower' : Bound .closed α}
+--     (h : UpwardEnumerable.succ? lower = some lower') :
+--     init? lower' = (init? lower).bind UpwardEnumerable.succ? := by
+--   cases h : init? lower <;> rename_i ilower <;> cases h' : init? lower' <;> rename_i ilower'
+--   · simp
+--   · simp [init?] at h
+--   · simp [init?] at h'
+--   · simp_all [init?]
+
+-- @[deprecated BoundedUpwardEnumerable.init?_succ?_closed (since := "2025-08-22")]
+-- public theorem BoundedUpwardEnumerable.Closed.init?_succ [UpwardEnumerable α]
+--     [LawfulUpwardEnumerable α] {lower lower' : Bound .closed α}
+--     (h : UpwardEnumerable.succ? lower = some lower') :
+--     init? lower' = (init? lower).bind UpwardEnumerable.succ? :=
+--   init?_succ?_closed h
+
+public theorem pairwise_toList_upwardEnumerableLt [LE α] [LT α] [DecidableLT α]
+    [UpwardEnumerable α] [LawfulUpwardEnumerable α] [LawfulUpwardEnumerableLT α]
+    [Rxo.IsAlwaysFinite α] [LawfulUpwardEnumerable α] :
+    r.toList.Pairwise (fun a b => UpwardEnumerable.LT a b) := by
+  rw [Internal.toList_eq_toList_iter]
+  apply Rxo.Iterator.pairwise_toList_upwardEnumerableLt
+
+public theorem pairwise_toList_ne [LE α] [LT α] [DecidableLT α]
+    [UpwardEnumerable α] [LawfulUpwardEnumerable α] [LawfulUpwardEnumerableLT α]
+    [Rxo.IsAlwaysFinite α] [LawfulUpwardEnumerable α] :
+    r.toList.Pairwise (fun a b => a ≠ b) :=
+  List.Pairwise.imp (fun hlt => UpwardEnumerable.ne_of_lt hlt) pairwise_toList_upwardEnumerableLt
+
+public theorem pairwise_toList_lt [LE α] [LT α] [DecidableLT α]
+    [UpwardEnumerable α] [LawfulUpwardEnumerable α] [LawfulUpwardEnumerableLT α]
+    [Rxo.IsAlwaysFinite α] [LawfulUpwardEnumerable α] :
+    r.toList.Pairwise (fun a b => a < b) :=
+  List.Pairwise.imp
+    (fun hlt => (LawfulUpwardEnumerableLT.lt_iff ..).mpr hlt) pairwise_toList_upwardEnumerableLt
+
+public theorem pairwise_toList_le [LE α] [LT α] [DecidableLT α]
+    [UpwardEnumerable α] [LawfulUpwardEnumerable α] [LawfulUpwardEnumerableLT α]
+    [LawfulUpwardEnumerableLE α] [Rxo.IsAlwaysFinite α] [LawfulUpwardEnumerable α] :
+    r.toList.Pairwise (fun a b => a ≤ b) :=
+  pairwise_toList_upwardEnumerableLt
+    |> List.Pairwise.imp UpwardEnumerable.le_of_lt
+    |> List.Pairwise.imp (fun hle => (UpwardEnumerable.le_iff ..).mpr hle)
+
+-- public theorem mem_Rco_succ_succ_iff [LE α] [DecidableLE α] [UpwardEnumerable α]
+--     [LinearlyUpwardEnumerable α] [LawfulUpwardEnumerableLE α] [InfinitelyUpwardEnumerable α]
+--     [HasFiniteRanges .open α] [LawfulUpwardEnumerable α] [LawfulOpenUpperBound α]
+--     {lower : Bound .closed α} {upper : Bound .open α} {a : α} :
+--     (a ∈ (succ lower)...(succ upper)) ↔ ∃ a', a = succ a' ∧ a' ∈ lower...upper := by
+--   simp [Membership.mem, LawfulUpwardEnumerableLowerBound.isSatisfied_iff,
+--     init?, LawfulOpenUpperBound.isSatisfied_iff_le]
+--   rw [← Option.some_get (InfinitelyUpwardEnumerable.isSome_succ? _)]
+--   simp only [Option.some.injEq, ← UpwardEnumerable.succ.eq_def]
+--   simp
+--   constructor
+--   · rintro ⟨⟨n, hn⟩, h⟩
+--     rw [succMany?_eq_some_iff_succMany, ← succMany_one, ← succMany_add, Nat.add_comm, succMany_add,
+--       succMany_one] at hn
+--     rw [← hn]
+--     refine ⟨succMany n lower, rfl, ?_, ?_⟩
+--     · exact ⟨n, by simp [succMany_eq_get]⟩
+--     · obtain ⟨m, hm⟩ := h
+--       refine ⟨m, ?_⟩
+--       rw [succMany?_eq_some_iff_succMany] at hm ⊢
+--       rwa [← hn, ← succMany_one, ← succMany_add, Nat.add_comm, succMany_add, succMany_one,
+--         succ_eq_succ_iff] at hm
+--   · rintro ⟨a', rfl, hl, hu⟩
+--     simp [UpwardEnumerable.succ_le_succ_iff, UpwardEnumerable.succ_lt_succ_iff]
+--     exact ⟨hl, hu⟩
+
+public theorem mem_succ_succ_iff [LE α] [LT α] [DecidableLT α] [UpwardEnumerable α]
+    [LinearlyUpwardEnumerable α] [LawfulUpwardEnumerableLT α] [LawfulUpwardEnumerableLE α]
+    [InfinitelyUpwardEnumerable α] [Rxo.IsAlwaysFinite α] [LawfulUpwardEnumerable α] {lo hi a : α} :
+    (a ∈ (succ lo)...(succ hi)) ↔ ∃ a', a = succ a' ∧ a' ∈ lo...hi := by
+  simp [Membership.mem, LawfulUpwardEnumerableLT.lt_iff, LawfulUpwardEnumerableLE.le_iff]
+  constructor
+  · intro h
+    obtain ⟨a', rfl, ha'⟩ := UpwardEnumerable.exists_of_succ_le h.1
+    exact ⟨a', rfl, ha', UpwardEnumerable.succ_lt_succ_iff.mp h.2⟩
+  · rintro ⟨a', rfl, hl, hu⟩
+    simp only [UpwardEnumerable.succ_le_succ_iff, UpwardEnumerable.succ_lt_succ_iff]
+    exact ⟨hl, hu⟩
+
+public theorem succ_mem_succ_succ_iff [LE α] [LT α] [DecidableLT α] [UpwardEnumerable α]
+    [LinearlyUpwardEnumerable α] [LawfulUpwardEnumerableLE α] [LawfulUpwardEnumerableLT α]
+    [InfinitelyUpwardEnumerable α] [Rxo.IsAlwaysFinite α] [LawfulUpwardEnumerable α] {lo hi a : α} :
+    (succ a ∈ (succ lo)...(succ hi)) ↔ a ∈ lo...hi := by
+  simp [mem_succ_succ_iff, UpwardEnumerable.succ_inj]
+
+-- public theorem toList_Rco_succ_succ_eq_map [UpwardEnumerable α] [SupportsLowerBound .closed α]
+--     [LinearlyUpwardEnumerable α] [InfinitelyUpwardEnumerable α] [SupportsUpperBound .open α]
+--     [HasFiniteRanges .open α] [LawfulUpwardEnumerable α] [LawfulOpenUpperBound α]
+--     [LawfulUpwardEnumerableLowerBound .closed α] [LawfulUpwardEnumerableUpperBound .open α]
+--     {lower : Bound .closed α} {upper : Bound .open α} :
+--     ((succ lower)...(succ upper)).toList =
+--       (lower...upper).toList.map succ := by
+--   apply eq_of_pairwise_lt_of_mem_iff_mem (lt := UpwardEnumerable.LT) (asymm := ?_)
+--   · apply pairwise_toList_upwardEnumerableLt
+--   · apply List.Pairwise.map (R := UpwardEnumerable.LT) (S := UpwardEnumerable.LT)
+--     · intro a b
+--       exact UpwardEnumerable.succ_lt_succ_iff.mpr
+--     · apply pairwise_toList_upwardEnumerableLt
+--   · simp only [List.mem_map, mem_toList_iff_mem]
+--     intro a
+--     rw [mem_Rco_succ_succ_iff]
+--     constructor
+--     · rintro ⟨a, rfl, h⟩
+--       exact ⟨a, h, rfl⟩
+--     · rintro ⟨a, h, h'⟩
+--       exact ⟨_, h'.symm, h⟩
+--   · exact ⟨fun _ _ => UpwardEnumerable.not_gt_of_lt⟩
+
+public theorem toList_succ_succ_eq_map [LE α] [DecidableLE α] [LT α] [DecidableLT α]
+    [UpwardEnumerable α] [LinearlyUpwardEnumerable α] [LawfulUpwardEnumerableLE α]
+    [LawfulUpwardEnumerableLT α] [InfinitelyUpwardEnumerable α] [Rxo.IsAlwaysFinite α]
+    [LawfulUpwardEnumerable α] {lo hi : α} :
+    ((succ lo)...(succ hi)).toList =
+      (lo...hi).toList.map succ := by
+  apply eq_of_pairwise_lt_of_mem_iff_mem (lt := UpwardEnumerable.LT)
+  · exact pairwise_toList_upwardEnumerableLt
+  · apply List.Pairwise.map (R := UpwardEnumerable.LT) (S := UpwardEnumerable.LT)
+    · exact fun _ _ => UpwardEnumerable.succ_lt_succ_iff.mpr
+    · exact pairwise_toList_upwardEnumerableLt
+  · simp [List.mem_map, mem_toList_iff_mem, mem_succ_succ_iff, eq_comm, and_comm]
+
+public theorem forIn'_eq_forIn'_toList [LE α] [DecidableLE α] [LT α] [DecidableLT α]
+    [UpwardEnumerable α] [LawfulUpwardEnumerableLE α] [LawfulUpwardEnumerableLT α]
+    [Rxo.IsAlwaysFinite α] [LawfulUpwardEnumerable α]
+    {γ : Type u} {init : γ} {m : Type u → Type w} [Monad m] [LawfulMonad m]
+    {f : (a : α) → a ∈ r → γ → m (ForInStep γ)} :
+    ForIn'.forIn' r init f =
+      ForIn'.forIn' r.toList init (fun a ha acc => f a (mem_toList_iff_mem.mp ha) acc) := by
+  simp [Internal.forIn'_eq_forIn'_iter, Internal.toList_eq_toList_iter,
+    Iter.forIn'_eq_forIn'_toList]
+
+public theorem forIn'_toList_eq_forIn' [LE α] [DecidableLE α] [LT α] [DecidableLT α]
+    [UpwardEnumerable α] [LawfulUpwardEnumerableLE α] [LawfulUpwardEnumerableLT α]
+    [Rxo.IsAlwaysFinite α] [LawfulUpwardEnumerable α]
+    {γ : Type u} {init : γ} {m : Type u → Type w} [Monad m] [LawfulMonad m]
+    {f : (a : α) → _ → γ → m (ForInStep γ)} :
+    ForIn'.forIn' r.toList init f =
+      ForIn'.forIn' r init (fun a ha acc => f a (mem_toList_iff_mem.mpr ha) acc) := by
+  simp [forIn'_eq_forIn'_toList]
+
+public theorem mem_of_mem_Roo [LE α] [LT α] [UpwardEnumerable α]
+    [LawfulUpwardEnumerableLE α] [LawfulUpwardEnumerableLT α] [Rxo.IsAlwaysFinite α]
+    [LawfulUpwardEnumerable α] {a b : α} (hrb : r.lower ≤ b) (hmem : a ∈ b<...r.upper) :
+    a ∈ r := by
+  haveI := UpwardEnumerable.instLETransOfLawfulUpwardEnumerableLE (α := α)
+  refine ⟨le_trans hrb ?_, hmem.2⟩
+  simp only [Membership.mem, LawfulUpwardEnumerableLE.le_iff, LawfulUpwardEnumerableLT.lt_iff] at hmem ⊢
+  exact UpwardEnumerable.le_of_lt hmem.1
+
+-- public theorem SupportsLowerBound.isSatisfied_init? {sl} [UpwardEnumerable α]
+--     [SupportsLowerBound sl α] [BoundedUpwardEnumerable sl α] [LawfulUpwardEnumerable α]
+--     [LawfulUpwardEnumerableLowerBound sl α]
+--     {bound : Bound sl α} {a : α} (h : init? bound = some a) :
+--     SupportsLowerBound.IsSatisfied bound a := by
+--   simp only [LawfulUpwardEnumerableLowerBound.isSatisfied_iff]
+--   exact ⟨a, h, UpwardEnumerable.le_refl _⟩
+
+public theorem forIn'_eq_match_Roo [LE α] [DecidableLE α] [LT α] [DecidableLT α]
+    [UpwardEnumerable α] [LawfulUpwardEnumerableLT α] [LawfulUpwardEnumerableLE α]
+    [Rxo.IsAlwaysFinite α] [LawfulUpwardEnumerable α]
+    {m : Type u → Type w} [Monad m] [LawfulMonad m]
+    {γ : Type u} {init : γ} {f : (a : α) → _ → γ → m (ForInStep γ)} :
+    ForIn'.forIn' r init f = if hu : r.lower < r.upper then do
+        have hle : r.lower ≤ r.lower := by
+          simpa [UpwardEnumerable.le_iff] using UpwardEnumerable.le_refl _
+        match ← f r.lower ⟨hle, hu⟩ init with
+        | .yield c =>
+          ForIn'.forIn' (α := α) (β := γ) (r.lower<...r.upper) c
+            (fun a ha acc => f a (mem_of_mem_Roo hle ha) acc)
+        | .done c => return c
+      else
+        return init := by
+  apply Eq.symm
+  rw [Internal.forIn'_eq_forIn'_iter, Iter.forIn'_eq_match_step]
+  simp only [Rxo.Iterator.step_eq_step, Rxo.Iterator.step, Internal.iter]
+  split
+  · apply bind_congr; intro step
+    split <;> simp [Roo.Internal.forIn'_eq_forIn'_iter, Roo.Internal.iter]
+  · simp
+
+public theorem isEmpty_iff_forall_not_mem [LE α] [LT α] [DecidableLT α] [UpwardEnumerable α]
+    [Rxo.HasSize α] [Rxo.LawfulHasSize α] [LawfulUpwardEnumerableLE α]
+    [LawfulUpwardEnumerableLT α] [Rxo.IsAlwaysFinite α]
+    [LawfulUpwardEnumerable α] :
+    r.isEmpty ↔ ∀ a, ¬ a ∈ r := by
+  simp only [isEmpty, decide_eq_true_eq]
+  constructor
+  · rintro h a ⟨hl, hu⟩
+    simp only [UpwardEnumerable.le_iff, UpwardEnumerable.lt_iff] at h hl hu
+    exact h.elim (UpwardEnumerable.lt_of_le_of_lt hl hu)
+  · intro h hi
+    refine h r.lower ⟨?_, hi⟩
+    simpa [UpwardEnumerable.le_iff] using UpwardEnumerable.le_refl _
+
+end Rco
+
+namespace Rci
+
+variable {r : Rci α}
+
+public theorem toList_eq_match [LE α] [UpwardEnumerable α]
+    [LawfulUpwardEnumerable α] [Rxi.IsAlwaysFinite α] [LawfulUpwardEnumerable α] :
+    r.toList = r.lower :: (r.lower<...*).toList := by
+  rw [Internal.toList_eq_toList_iter, Rxi.Iterator.toList_eq_match]; rfl
+
+public theorem toList_ne_nil [LE α] [UpwardEnumerable α]
+    [LawfulUpwardEnumerable α] [Rxi.IsAlwaysFinite α]
+    [LawfulUpwardEnumerable α] :
+    r.toList ≠ [] := by
+  rw [Internal.toList_eq_toList_iter, Rxi.Iterator.toList_eq_match, Internal.iter]
+  simp
+
+public theorem mem_toList_iff_mem [LE α] [DecidableLE α] [UpwardEnumerable α]
+    [LawfulUpwardEnumerable α] [LawfulUpwardEnumerableLE α]
+    [Rxi.IsAlwaysFinite α] [LawfulUpwardEnumerable α] {a : α} : a ∈ r.toList ↔ a ∈ r := by
+  rw [Internal.toList_eq_toList_iter, Iter.mem_toList_iff_isPlausibleIndirectOutput,
+    Internal.isPlausibleIndirectOutput_iter_iff]
+
+-- public theorem BoundedUpwardEnumerable.init?_succ?_closed [UpwardEnumerable α]
+--     [LawfulUpwardEnumerable α] {lower lower' : Bound .closed α}
+--     (h : UpwardEnumerable.succ? lower = some lower') :
+--     init? lower' = (init? lower).bind UpwardEnumerable.succ? := by
+--   cases h : init? lower <;> rename_i ilower <;> cases h' : init? lower' <;> rename_i ilower'
+--   · simp
+--   · simp [init?] at h
+--   · simp [init?] at h'
+--   · simp_all [init?]
+
+-- @[deprecated BoundedUpwardEnumerable.init?_succ?_closed (since := "2025-08-22")]
+-- public theorem BoundedUpwardEnumerable.Closed.init?_succ [UpwardEnumerable α]
+--     [LawfulUpwardEnumerable α] {lower lower' : Bound .closed α}
+--     (h : UpwardEnumerable.succ? lower = some lower') :
+--     init? lower' = (init? lower).bind UpwardEnumerable.succ? :=
+--   init?_succ?_closed h
+
+public theorem pairwise_toList_upwardEnumerableLt [LE α]
+    [UpwardEnumerable α] [LawfulUpwardEnumerable α] [Rxi.IsAlwaysFinite α] [LawfulUpwardEnumerable α] :
+    r.toList.Pairwise (fun a b => UpwardEnumerable.LT a b) := by
+  rw [Internal.toList_eq_toList_iter]
+  apply Rxi.Iterator.pairwise_toList_upwardEnumerableLt
+
+public theorem pairwise_toList_ne [LE α]
+    [UpwardEnumerable α] [LawfulUpwardEnumerable α] [Rxi.IsAlwaysFinite α] [LawfulUpwardEnumerable α] :
+    r.toList.Pairwise (fun a b => a ≠ b) :=
+  List.Pairwise.imp (fun hlt => UpwardEnumerable.ne_of_lt hlt) pairwise_toList_upwardEnumerableLt
+
+public theorem pairwise_toList_lt [LE α] [LT α]
+    [UpwardEnumerable α] [LawfulUpwardEnumerable α]
+    [LawfulUpwardEnumerableLT α] [Rxi.IsAlwaysFinite α] [LawfulUpwardEnumerable α] :
+    r.toList.Pairwise (fun a b => a < b) :=
+  List.Pairwise.imp
+    (fun hlt => (LawfulUpwardEnumerableLT.lt_iff ..).mpr hlt) pairwise_toList_upwardEnumerableLt
+
+public theorem pairwise_toList_le [LE α]
+    [UpwardEnumerable α] [LawfulUpwardEnumerable α] [LawfulUpwardEnumerableLE α]
+    [Rxi.IsAlwaysFinite α] [LawfulUpwardEnumerable α] :
+    r.toList.Pairwise (fun a b => a ≤ b) :=
+  pairwise_toList_upwardEnumerableLt
+    |> List.Pairwise.imp UpwardEnumerable.le_of_lt
+    |> List.Pairwise.imp (fun hle => (UpwardEnumerable.le_iff ..).mpr hle)
+
+-- public theorem mem_Rci_succ_succ_iff [LE α] [DecidableLE α] [UpwardEnumerable α]
+--     [LinearlyUpwardEnumerable α] [LawfulUpwardEnumerableLE α] [InfinitelyUpwardEnumerable α]
+--     [HasFiniteRanges .open α] [LawfulUpwardEnumerable α] [LawfulOpenUpperBound α]
+--     {lower : Bound .closed α} {upper : Bound .open α} {a : α} :
+--     (a ∈ (succ lower)...(succ upper)) ↔ ∃ a', a = succ a' ∧ a' ∈ lower...upper := by
+--   simp [Membership.mem, LawfulUpwardEnumerableLowerBound.isSatisfied_iff,
+--     init?, LawfulOpenUpperBound.isSatisfied_iff_le]
+--   rw [← Option.some_get (InfinitelyUpwardEnumerable.isSome_succ? _)]
+--   simp only [Option.some.injEq, ← UpwardEnumerable.succ.eq_def]
+--   simp
+--   constructor
+--   · rintro ⟨⟨n, hn⟩, h⟩
+--     rw [succMany?_eq_some_iff_succMany, ← succMany_one, ← succMany_add, Nat.add_comm, succMany_add,
+--       succMany_one] at hn
+--     rw [← hn]
+--     refine ⟨succMany n lower, rfl, ?_, ?_⟩
+--     · exact ⟨n, by simp [succMany_eq_get]⟩
+--     · obtain ⟨m, hm⟩ := h
+--       refine ⟨m, ?_⟩
+--       rw [succMany?_eq_some_iff_succMany] at hm ⊢
+--       rwa [← hn, ← succMany_one, ← succMany_add, Nat.add_comm, succMany_add, succMany_one,
+--         succ_eq_succ_iff] at hm
+--   · rintro ⟨a', rfl, hl, hu⟩
+--     simp [UpwardEnumerable.succ_le_succ_iff, UpwardEnumerable.succ_lt_succ_iff]
+--     exact ⟨hl, hu⟩
+
+public theorem mem_succ_iff [LE α] [UpwardEnumerable α]
+    [LinearlyUpwardEnumerable α] [LawfulUpwardEnumerableLE α]
+    [InfinitelyUpwardEnumerable α] [Rxi.IsAlwaysFinite α] [LawfulUpwardEnumerable α] {lo a : α} :
+    (a ∈ (succ lo)...*) ↔ ∃ a', a = succ a' ∧ a' ∈ lo...* := by
+  simp [Membership.mem, LawfulUpwardEnumerableLE.le_iff]
+  constructor
+  · intro h
+    obtain ⟨a', rfl, ha'⟩ := UpwardEnumerable.exists_of_succ_le h
+    exact ⟨a', rfl, UpwardEnumerable.succ_le_succ_iff.mp h⟩
+  · rintro ⟨a', rfl, hl, hu⟩
+    simp only [UpwardEnumerable.succ_le_succ_iff, UpwardEnumerable.succ_le_succ_iff]
+    exact ⟨hl, hu⟩
+
+public theorem succ_mem_succ_succ_iff [LE α] [UpwardEnumerable α]
+    [LinearlyUpwardEnumerable α] [LawfulUpwardEnumerableLE α]
+    [InfinitelyUpwardEnumerable α] [Rxi.IsAlwaysFinite α] [LawfulUpwardEnumerable α] {lo a : α} :
+    (succ a ∈ (succ lo)...*) ↔ a ∈ lo...* := by
+  simp [mem_succ_iff, UpwardEnumerable.succ_inj]
+
+-- public theorem toList_Rci_succ_succ_eq_map [UpwardEnumerable α] [SupportsLowerBound .closed α]
+--     [LinearlyUpwardEnumerable α] [InfinitelyUpwardEnumerable α] [SupportsUpperBound .open α]
+--     [HasFiniteRanges .open α] [LawfulUpwardEnumerable α] [LawfulOpenUpperBound α]
+--     [LawfulUpwardEnumerableLowerBound .closed α] [LawfulUpwardEnumerableUpperBound .open α]
+--     {lower : Bound .closed α} {upper : Bound .open α} :
+--     ((succ lower)...(succ upper)).toList =
+--       (lower...upper).toList.map succ := by
+--   apply eq_of_pairwise_lt_of_mem_iff_mem (lt := UpwardEnumerable.LT) (asymm := ?_)
+--   · apply pairwise_toList_upwardEnumerableLt
+--   · apply List.Pairwise.map (R := UpwardEnumerable.LT) (S := UpwardEnumerable.LT)
+--     · intro a b
+--       exact UpwardEnumerable.succ_lt_succ_iff.mpr
+--     · apply pairwise_toList_upwardEnumerableLt
+--   · simp only [List.mem_map, mem_toList_iff_mem]
+--     intro a
+--     rw [mem_Rci_succ_succ_iff]
+--     constructor
+--     · rintro ⟨a, rfl, h⟩
+--       exact ⟨a, h, rfl⟩
+--     · rintro ⟨a, h, h'⟩
+--       exact ⟨_, h'.symm, h⟩
+--   · exact ⟨fun _ _ => UpwardEnumerable.not_gt_of_lt⟩
+
+public theorem toList_succ_succ_eq_map [LE α] [DecidableLE α]
+    [UpwardEnumerable α] [LinearlyUpwardEnumerable α] [LawfulUpwardEnumerableLE α]
+    [InfinitelyUpwardEnumerable α] [Rxi.IsAlwaysFinite α]
+    [LawfulUpwardEnumerable α] {lo : α} :
+    ((succ lo)...*).toList = (lo...*).toList.map succ := by
+  apply eq_of_pairwise_lt_of_mem_iff_mem (lt := UpwardEnumerable.LT)
+  · exact pairwise_toList_upwardEnumerableLt
+  · apply List.Pairwise.map (R := UpwardEnumerable.LT) (S := UpwardEnumerable.LT)
+    · exact fun _ _ => UpwardEnumerable.succ_lt_succ_iff.mpr
+    · exact pairwise_toList_upwardEnumerableLt
+  · simp [List.mem_map, mem_toList_iff_mem, mem_succ_iff, eq_comm, and_comm]
+
+public theorem forIn'_eq_forIn'_toList [LE α] [DecidableLE α]
+    [UpwardEnumerable α] [LawfulUpwardEnumerableLE α]
+    [Rxi.IsAlwaysFinite α] [LawfulUpwardEnumerable α]
+    {γ : Type u} {init : γ} {m : Type u → Type w} [Monad m] [LawfulMonad m]
+    {f : (a : α) → a ∈ r → γ → m (ForInStep γ)} :
+    ForIn'.forIn' r init f =
+      ForIn'.forIn' r.toList init (fun a ha acc => f a (mem_toList_iff_mem.mp ha) acc) := by
+  simp [Internal.forIn'_eq_forIn'_iter, Internal.toList_eq_toList_iter,
+    Iter.forIn'_eq_forIn'_toList]
+
+public theorem forIn'_toList_eq_forIn' [LE α] [DecidableLE α]
+    [UpwardEnumerable α] [LawfulUpwardEnumerableLE α]
+    [Rxi.IsAlwaysFinite α] [LawfulUpwardEnumerable α]
+    {γ : Type u} {init : γ} {m : Type u → Type w} [Monad m] [LawfulMonad m]
+    {f : (a : α) → _ → γ → m (ForInStep γ)} :
+    ForIn'.forIn' r.toList init f =
+      ForIn'.forIn' r init (fun a ha acc => f a (mem_toList_iff_mem.mpr ha) acc) := by
+  simp [forIn'_eq_forIn'_toList]
+
+public theorem mem_of_mem_Roi [LE α] [LT α] [UpwardEnumerable α]
+    [LawfulUpwardEnumerableLE α] [LawfulUpwardEnumerableLT α] [Rxi.IsAlwaysFinite α]
+    [LawfulUpwardEnumerable α] {a b : α} (hrb : r.lower ≤ b) (hmem : a ∈ b<...*) :
+    a ∈ r := by
+  haveI := UpwardEnumerable.instLETransOfLawfulUpwardEnumerableLE (α := α)
+  refine le_trans hrb ?_
+  simp only [Membership.mem, LawfulUpwardEnumerableLE.le_iff, LawfulUpwardEnumerableLT.lt_iff] at hmem ⊢
+  exact UpwardEnumerable.le_of_lt hmem
+
+-- public theorem SupportsLowerBound.isSatisfied_init? {sl} [UpwardEnumerable α]
+--     [SupportsLowerBound sl α] [BoundedUpwardEnumerable sl α] [LawfulUpwardEnumerable α]
+--     [LawfulUpwardEnumerableLowerBound sl α]
+--     {bound : Bound sl α} {a : α} (h : init? bound = some a) :
+--     SupportsLowerBound.IsSatisfied bound a := by
+--   simp only [LawfulUpwardEnumerableLowerBound.isSatisfied_iff]
+--   exact ⟨a, h, UpwardEnumerable.le_refl _⟩
+
+public theorem forIn'_eq_match_Roi [LE α] [DecidableLE α] [LT α] [DecidableLT α]
+    [UpwardEnumerable α] [LawfulUpwardEnumerableLT α] [LawfulUpwardEnumerableLE α]
+    [Rxi.IsAlwaysFinite α] [LawfulUpwardEnumerable α]
+    {m : Type u → Type w} [Monad m] [LawfulMonad m]
+    {γ : Type u} {init : γ} {f : (a : α) → _ → γ → m (ForInStep γ)} :
+    ForIn'.forIn' r init f = do
+      have hle : r.lower ≤ r.lower := by
+        simpa [UpwardEnumerable.le_iff] using UpwardEnumerable.le_refl _
+      match ← f r.lower hle init with
+      | .yield c =>
+        ForIn'.forIn' (α := α) (β := γ) (r.lower<...*) c
+          (fun a ha acc => f a (mem_of_mem_Roi hle ha) acc)
+      | .done c => return c := by
+  apply Eq.symm
+  rw [Internal.forIn'_eq_forIn'_iter, Iter.forIn'_eq_match_step]
+  simp only [Rxi.Iterator.step_eq_step, Rxi.Iterator.step, Internal.iter]
+  apply bind_congr; intro step
+  split <;> simp [Roi.Internal.forIn'_eq_forIn'_iter, Roi.Internal.iter]
+
+public theorem isEmpty_iff_forall_not_mem [LE α] [UpwardEnumerable α]
+    [Rxi.HasSize α] [Rxi.LawfulHasSize α] [LawfulUpwardEnumerableLE α] [Rxi.IsAlwaysFinite α]
+    [LawfulUpwardEnumerable α] :
+    r.isEmpty ↔ ∀ a, ¬ a ∈ r := by
+  simp only [isEmpty, Bool.false_eq_true, false_iff, Classical.not_forall, Classical.not_not]
+  exact ⟨r.lower, by simpa [← UpwardEnumerable.le_iff] using UpwardEnumerable.le_refl (α := α) _⟩
+
+end Rci
+
+private theorem Internal.iter_Roc_eq_iter_Rcc_of_isSome_succ?
+    [LE α] [UpwardEnumerable α] [LawfulUpwardEnumerable α] {lo hi : α}
+    (h : (UpwardEnumerable.succ? lo).isSome) :
+    Roc.Internal.iter (lo<...=hi) =
+      Rcc.Internal.iter ((UpwardEnumerable.succ? lo |>.get h)...=hi) := by
+  simp [Roc.Internal.iter, Rcc.Internal.iter]
+
+public theorem toList_Roc_eq_toList_Rcc_of_isSome_succ? [LE α] [DecidableLE α] [UpwardEnumerable α]
+    [LawfulUpwardEnumerable α] [LawfulUpwardEnumerableLE α] [Rxc.IsAlwaysFinite α]
+    [LawfulUpwardEnumerable α]
+    {lo hi : α} (h : (UpwardEnumerable.succ? lo).isSome) :
+    (lo<...=hi).toList =
+      ((UpwardEnumerable.succ? lo |>.get h)...=hi).toList := by
+  simp [Rcc.Internal.toList_eq_toList_iter, Roc.Internal.toList_eq_toList_iter,
+    Internal.iter_Roc_eq_iter_Rcc_of_isSome_succ?, h]
+
+private theorem Internal.iter_Roo_eq_iter_Rco_of_isSome_succ?
+    [LE α] [LT α] [UpwardEnumerable α]
+    [LawfulUpwardEnumerable α] {lo hi : α} (h : (UpwardEnumerable.succ? lo).isSome) :
+    Roo.Internal.iter (lo<...hi) =
+      Rco.Internal.iter ((UpwardEnumerable.succ? lo |>.get h)...hi) := by
+  simp [Roo.Internal.iter, Rco.Internal.iter]
+
+public theorem toList_Roo_eq_toList_Rco_of_isSome_succ? [LE α] [DecidableLE α]
+    [LT α] [DecidableLT α] [UpwardEnumerable α]
+    [LawfulUpwardEnumerable α] [LawfulUpwardEnumerableLE α] [LawfulUpwardEnumerableLT α]
+    [Rxo.IsAlwaysFinite α] [LawfulUpwardEnumerable α]
+    {lo hi : α} (h : (UpwardEnumerable.succ? lo).isSome) :
+    (lo<...hi).toList =
+      ((UpwardEnumerable.succ? lo |>.get h)...hi).toList := by
+  simp [Rco.Internal.toList_eq_toList_iter, Roo.Internal.toList_eq_toList_iter,
+    Internal.iter_Roo_eq_iter_Rco_of_isSome_succ?, h]
+
+private theorem Internal.iter_Roi_eq_iter_Rci_of_isSome_succ?
+    [LE α] [LT α] [UpwardEnumerable α]
+    [LawfulUpwardEnumerable α] {lo : α} (h : (UpwardEnumerable.succ? lo).isSome) :
+    Roi.Internal.iter (lo<...*) =
+      Rci.Internal.iter ((UpwardEnumerable.succ? lo |>.get h)...*) := by
+  simp [Roi.Internal.iter, Rci.Internal.iter]
+
+public theorem toList_Roi_eq_toList_Rci_of_isSome_succ? [LE α] [DecidableLE α]
+    [LT α] [DecidableLT α] [UpwardEnumerable α]
+    [LawfulUpwardEnumerable α] [LawfulUpwardEnumerableLE α] [LawfulUpwardEnumerableLT α]
+    [Rxi.IsAlwaysFinite α] [LawfulUpwardEnumerable α]
+    {lo : α} (h : (UpwardEnumerable.succ? lo).isSome) :
+    (lo<...*).toList = ((UpwardEnumerable.succ? lo |>.get h)...*).toList := by
+  simp [Rci.Internal.toList_eq_toList_iter, Roi.Internal.toList_eq_toList_iter,
+    Internal.iter_Roi_eq_iter_Rci_of_isSome_succ?, h]
+
+end Std
